coq/lib/P4cub/Semantics/Dynamic/BigStep/Semantics.v
@@ -123,7 +123,7 @@ Variant signal : Set :=
 Variant Embed_signal : signal -> Value.signal -> Prop :=
 | embed_cont : Embed_signal Cont Value.SContinue
 | embed_exit : Embed_signal Exit Value.SExit
-| embed_rjct : Embed_signal Rjct (Value.SReject "")
+| embed_rjct x : Embed_signal Rjct (Value.SReject x)
 | embed_acpt : Embed_signal Acpt Value.SContinue (* TODO: look at tofino, maybe return here *)
 | embed_rtrn_none : Embed_signal (Rtrn None) Value.SReturnNull
 | embed_rtrn_some v v' :
@@ -377,7 +377,9 @@ Inductive stm_big_step
   (** Evaluate table key. *)
   Forall2 (exp_big_step ϵ₂) (map fst key) vs ->
   (** Evaluate table entries. *)
-  Forall3 table_entry_big_step (extern_get_entries ψ []) pats arefs ->
+  Forall3 table_entry_big_step (extern_get_entries Ψ.(extrn_state) []) pats arefs ->
+  (** Embed table key *)
+  Forall2 Embed vs light_vals ->
   (** Embed p4cub patterns in p4light val sets. *)
   Forall2 embed_pat_valset pats light_sets ->
   (** Get action reference from control-plane with control-plane arguments. *)
